working on coq proof for the correctness of PROC interpreter

PROC/proof.v
@@ -8,26 +8,31 @@ Inductive expression : Set :=
 | If : expression -> expression -> expression -> expression
 | Var : string -> expression
 | Let : string -> expression -> expression -> expression
+| Proc : string -> expression -> expression
+| Call : expression -> expression -> expression
 .
 
-Inductive expval : Set :=
-| Num : Z -> expval
-| Bool : bool -> expval
-.
-
-Definition environment := string -> option expval.
-Definition empty_env : environment := (fun _ => None).
-Definition extend_env (x : string) (v : expval) (env : environment) :=
+Definition environment (A : Type) := string -> option A.
+Definition empty_env {A : Type} : environment A := (fun _ => None).
+Definition extend_env {A : Type} (x : string) (v : A) (env : environment A) :=
     fun y => if string_dec x y then Some v else env y.
 
-Inductive value_of_rel : expression -> environment -> expval -> Prop :=
+Inductive expval : Type :=
+| Num : Z -> expval
+| Bool : bool -> expval
+| Clo : string -> expression -> environment expval -> expval
+.
+
+Inductive value_of_rel : expression -> environment expval -> expval -> Prop :=
 | VConst : forall num env, value_of_rel (Const num) env (Num (Z.of_nat num))
 | VDiff : forall exp1 exp2 num1 num2 env, value_of_rel exp1 env (Num num1) -> value_of_rel exp2 env (Num num2) -> value_of_rel (Diff exp1 exp2) env (Num (num1 - num2))
 | VIsZero : forall exp1 num1 env, value_of_rel exp1 env (Num num1) -> value_of_rel (IsZero exp1) env (Bool (Z.eqb num1 0))
 | VIfTrue : forall exp1 exp2 exp3 val2 env, value_of_rel exp1 env (Bool true) -> value_of_rel exp2 env val2 -> value_of_rel (If exp1 exp2 exp3) env val2
 | VIfFalse : forall exp1 exp2 exp3 val3 env, value_of_rel exp1 env (Bool false) -> value_of_rel exp3 env val3 -> value_of_rel (If exp1 exp2 exp3) env val3
 | VVar : forall var env val, env var = Some val -> value_of_rel (Var var) env val
-| VLet :forall var exp1 body env val1 valb, value_of_rel exp1 env val1 -> value_of_rel body (extend_env var val1 env) valb -> value_of_rel (Let var exp1 body) env valb
+| VLet : forall var exp1 body env val1 valb, value_of_rel exp1 env val1 -> value_of_rel body (extend_env var val1 env) valb -> value_of_rel (Let var exp1 body) env valb
+| VProc : forall var body env, value_of_rel (Proc var body) env (Clo var body env)
+| VCall : forall rator rand env var body saved_env rand_val valb, value_of_rel rator env (Clo var body saved_env) -> value_of_rel rand env rand_val -> value_of_rel body (extend_env var rand_val saved_env) valb -> value_of_rel (Call rator rand) env valb
 .
 
 Notation "x <- e1 ; e2" :=
@@ -37,33 +42,46 @@ Notation "x <- e1 ; e2" :=
     end)
 (right associativity, at level 60).
 
-Fixpoint value_of (exp : expression) (env : environment) : option expval :=
-    match exp with
-    | Const num => Some (Num (Z.of_nat num))
-    | Diff exp1 exp2 =>
-            val1 <- value_of exp1 env;
-            val2 <- value_of exp2 env;
-            match (val1, val2) with
-            | (Num num1, Num num2) => Some (Num (num1 - num2))
-            | _ => None
+Function value_of (exp : expression) (env : environment expval) (fuel : nat) : option expval :=
+    match fuel with
+    | O => None
+    | S fuel' =>
+            match exp with
+            | Const num => Some (Num (Z.of_nat num))
+            | Diff exp1 exp2 =>
+                    val1 <- value_of exp1 env fuel';
+                    val2 <- value_of exp2 env fuel';
+                    match (val1, val2) with
+                    | (Num num1, Num num2) => Some (Num (num1 - num2))
+                    | _ => None
+                    end
+            | IsZero exp1 =>
+                    val1 <- value_of exp1 env fuel';
+                    match val1 with
+                    | Num num1 => Some (Bool (Z.eqb num1 0))
+                    | _ => None
+                    end
+            | If exp1 exp2 exp3 =>
+                    val1 <- value_of exp1 env fuel';
+                    match val1 with
+                    | Bool true => value_of exp2 env fuel'
+                    | Bool false => value_of exp3 env fuel'
+                    | _ => None
+                    end
+            | Var var => env var
+            | Let var exp1 body =>
+                    val1 <- value_of exp1 env fuel';
+                    value_of body (extend_env var val1 env) fuel'
+            | Proc var body => Some (Clo var body env)
+            | Call rator rand =>
+                    rator_val <- value_of rator env fuel';
+                    match rator_val with
+                    | Clo var body saved_env =>
+                            rand_val <- value_of rand env fuel';
+                            value_of body (extend_env var rand_val saved_env) fuel'
+                    | _ => None
+                    end
             end
-    | IsZero exp1 =>
-            val1 <- value_of exp1 env;
-            match val1 with
-            | Num num1 => Some (Bool (Z.eqb num1 0))
-            | _ => None
-            end
-    | If exp1 exp2 exp3 =>
-            val1 <- value_of exp1 env;
-            match val1 with
-            | Bool true => value_of exp2 env
-            | Bool false => value_of exp3 env
-            | _ => None
-            end
-    | Var var => env var
-    | Let var exp1 body =>
-            val1 <- value_of exp1 env;
-            value_of body (extend_env var val1 env)
     end.
 
 Lemma option_eq {T : Type} (p q : T) : Some p = Some q -> p = q.
@@ -72,44 +90,118 @@ Qed.
 
 Hint Constructors value_of_rel.
 
-Theorem value_of_soundness : forall exp env val, value_of exp env = Some val -> value_of_rel exp env val.
+Theorem value_of_soundness : forall exp env val, (exists fuel, value_of exp env fuel = Some val) -> value_of_rel exp env val.
+    intros.
+    destruct H as [ fuel H ].
+    generalize dependent val.
+    generalize dependent env.
+    generalize dependent fuel.
+    induction exp; intros; destruct fuel; try discriminate; simpl in H; eauto.
+        apply option_eq in H. rewrite <- H. auto.
+
+        destruct (value_of exp1 env fuel) eqn:?; try discriminate.
+        specialize (IHexp1 fuel env e).
+        destruct (value_of exp2 env fuel) eqn:?; try discriminate.
+        specialize (IHexp2 fuel env e0).
+        destruct e eqn:?; try discriminate.
+        destruct e0 eqn:?; try discriminate.
+        apply option_eq in H. rewrite <- H. auto.
+
+        destruct (value_of exp env fuel) eqn:?; try discriminate.
+        specialize (IHexp fuel env e).
+        destruct e eqn:?; try discriminate.
+        apply option_eq in H. rewrite <- H. auto.
+
+        destruct (value_of exp1 env fuel) eqn:?; try discriminate.
+        specialize (IHexp1 fuel env e).
+        destruct e; try discriminate.
+        destruct b. specialize (IHexp2 fuel env val). auto. specialize (IHexp3 fuel env val). auto.
+
+        destruct (value_of exp1 env fuel) eqn:?; try discriminate.
+        specialize (IHexp1 fuel env e).
+        specialize (IHexp2 fuel (extend_env s e env) val). eauto.
+
+        apply option_eq in H. rewrite <- H. auto.
+
+        destruct (value_of exp1 env fuel) eqn:?; try discriminate.
+        specialize (IHexp1 fuel env e).
+        destruct e; try discriminate.
+        destruct (value_of exp2 env fuel) eqn:?; try discriminate.
+        specialize (IHexp2 fuel env e1).
+Admitted.
+
+Lemma fuel_greater_than_zero : forall exp env fuel val, value_of exp env fuel = Some val -> fuel > O.
+    intros.
+    destruct fuel; try omega; discriminate.
+Qed.
+
+Lemma fuel_partial_order : forall exp env fuel val, value_of exp env fuel = Some val -> value_of exp env (S fuel) = Some val.
     intros.
     generalize dependent val.
     generalize dependent env.
-    induction exp; intros; eauto; simpl in H.
-        apply option_eq in H. rewrite <- H. auto.
+    generalize dependent fuel.
+    induction exp; intros; destruct fuel; try discriminate; simpl in H; eauto.
+        destruct (value_of exp1 env fuel) eqn:?; try discriminate.
+        specialize (IHexp1 fuel env e).
+        destruct (value_of exp2 env fuel) eqn:?; try discriminate.
+        specialize (IHexp2 fuel env e0).
+        destruct e eqn:?; try discriminate.
+        destruct e0 eqn:?; try discriminate.
+        apply option_eq in H. rewrite <- H.
+        apply IHexp1 in Heqo.
+        apply IHexp2 in Heqo0.
+        rewrite value_of_equation.
+        rewrite -> Heqo.
+        rewrite -> Heqo0.
+        auto.
 
-        destruct (value_of exp1 env) eqn:?; try discriminate.
-        specialize (IHexp1 env e). destruct (value_of exp2 env) eqn:?; try discriminate.
-        specialize (IHexp2 env e0). destruct e; try discriminate.
-        destruct e0; try discriminate.
-        apply option_eq in H. rewrite <- H. auto.
+        destruct (value_of exp env fuel) eqn:?; try discriminate.
+        specialize (IHexp fuel env e).
+        destruct e eqn:?; try discriminate.
+        apply option_eq in H. rewrite <- H.
+        apply IHexp in Heqo.
+        rewrite value_of_equation.
+        rewrite -> Heqo.
+        auto.
 
-        destruct (value_of exp env) eqn:?; try discriminate.
-        specialize (IHexp env e). destruct e; try discriminate.
-        apply option_eq in H. rewrite <- H. auto.
+        destruct (value_of exp1 env fuel) eqn:?; try discriminate.
+        specialize (IHexp1 fuel env e).
+        destruct e eqn:?; try discriminate.
+        apply IHexp1 in Heqo.
+        destruct b.
+            specialize (IHexp2 fuel env val). apply IHexp2 in H. rewrite value_of_equation. rewrite -> Heqo. auto.
+            specialize (IHexp3 fuel env val). apply IHexp3 in H. rewrite value_of_equation. rewrite -> Heqo. auto.
 
-        destruct (value_of exp1 env) eqn:?; try discriminate.
-        specialize (IHexp1 env e). destruct e; try discriminate.
-        destruct b; auto.
+        destruct (value_of exp1 env fuel) eqn:?; try discriminate.
+        specialize (IHexp1 fuel env e).
+        apply IHexp1 in Heqo.
+        specialize (IHexp2 fuel (extend_env s e env) val).
+        apply IHexp2 in H.
+        rewrite value_of_equation.
+        rewrite -> Heqo.
+        auto.
 
-        destruct (value_of exp1 env) eqn:?; try discriminate.
-        specialize (IHexp1 env e). specialize (IHexp2 (extend_env s e env) val). eauto.
-Qed.
+        destruct (value_of exp1 env fuel) eqn:?; try discriminate.
+        specialize (IHexp1 fuel env e).
+        apply IHexp1 in Heqo.
+        destruct e eqn:?; try discriminate.
+        destruct (value_of exp2 env fuel) eqn:?; try discriminate.
+        specialize (IHexp2 fuel env e2).
+        apply IHexp2 in Heqo0.
+        rewrite value_of_equation.
+        rewrite -> Heqo.
+        rewrite -> Heqo0.
+Admitted.
 
-Theorem value_of_completeness : forall exp env val, value_of_rel exp env val -> value_of exp env = Some val.
+Theorem value_of_completeness : forall exp env val, value_of_rel exp env val -> exists fuel, value_of exp env fuel = Some val.
     intros.
-    induction H; simpl; eauto.
-        rewrite -> IHvalue_of_rel1. rewrite -> IHvalue_of_rel2. auto.
-        rewrite -> IHvalue_of_rel. auto.
-        rewrite -> IHvalue_of_rel1. auto.
-        rewrite -> IHvalue_of_rel1. auto.
-        rewrite -> IHvalue_of_rel1. auto.
-Qed.
+    induction H.
+        exists (S O); auto.
 
-Theorem value_of_correctness : forall exp env val, value_of exp env = Some val <-> value_of_rel exp env val.
-    intros.
-    split.
-        apply value_of_soundness.
-        apply value_of_completeness.
-Qed.
+        destruct IHvalue_of_rel1 as [ fuel1 H1 ].
+        destruct IHvalue_of_rel2 as [ fuel2 H2 ].
+        exists (S (max fuel1 fuel2)).
+Abort.
+
+Theorem value_of_correctness : forall exp env val, (exists fuel, value_of exp env fuel = Some val) <-> value_of_rel exp env val.
+Abort.
